optimize mbufn and mbuf2S

thys/MFODL_Monitor_Devel/Monitor.thy
@@ -679,8 +679,19 @@ lift_definition mbuf_t_append :: "'a mbuf_t \<Rightarrow> 'a list \<Rightarrow> 
 
 notation mbuf_t_append (infixr "@@" 65)
 
+lift_definition mbuf_t_is_empty :: "'a mbuf_t \<Rightarrow> bool" is "\<lambda>xs. xs = []" .
+
 lift_definition mbuf_t_cases :: "'a mbuf_t \<Rightarrow> 'a option \<times> 'a mbuf_t" is
   "\<lambda>xs. case xs of [] \<Rightarrow> (None, xs) | y # ys \<Rightarrow> (Some y, ys)" .
+
+lemma Rep_mbuf_t_cases[simp]:
+  "mbuf_t_cases xs = (None, xs') \<Longrightarrow> Rep_mbuf_t xs = []"
+  "mbuf_t_cases xs = (None, xs') \<Longrightarrow> Rep_mbuf_t xs' = []"
+  "mbuf_t_cases xs = (Some x, xs') \<Longrightarrow> Rep_mbuf_t xs = x # Rep_mbuf_t xs'"
+  subgoal by transfer (auto split: option.splits list.splits)
+  subgoal by transfer (auto split: option.splits list.splits)
+  subgoal by transfer (auto split: option.splits list.splits)
+  done
 
 lemma mbuf_t_cases_size[termination_simp]: "(Some x, xs') = mbuf_t_cases xs \<Longrightarrow> size xs' < size xs"
   by transfer (auto split: list.splits)
@@ -688,8 +699,8 @@ lemma mbuf_t_cases_size[termination_simp]: "(Some x, xs') = mbuf_t_cases xs \<Lo
 type_synonym ts = nat
 
 type_synonym 'a mbuf2 = "'a table mbuf_t \<times> 'a table mbuf_t"
-type_synonym 'a mbufn = "'a table list list"
-type_synonym 'a mbuf2S = "'a table list \<times> 'a table list \<times> ts list \<times> bool"
+type_synonym 'a mbufn = "'a table mbuf_t list"
+type_synonym 'a mbuf2S = "'a table mbuf_t \<times> 'a table mbuf_t \<times> ts mbuf_t \<times> bool"
 type_synonym 'a msaux = "(ts \<times> 'a table) list"
 type_synonym 'a muaux = "(ts \<times> 'a table \<times> 'a table) list"
 type_synonym 'a mr\<delta>aux = "(ts \<times> (mregex, 'a table) mapping) list"
@@ -886,7 +897,7 @@ definition pred_mode_of :: "nat \<Rightarrow> Formula.trm list \<Rightarrow> pre
   "pred_mode_of n ts = (if is_copy_pattern n ts then Copy
     else if is_simple_pattern ts 0 then Simple else Match)"
 
-abbreviation (input) "init_mbuf2S \<equiv> ([], [], [], False)"
+abbreviation (input) "init_mbuf2S \<equiv> (mbuf_t_empty, mbuf_t_empty, mbuf_t_empty, False)"
 
 function (in maux) (sequential) minit0 :: "nat \<Rightarrow> Formula.formula \<Rightarrow> ('msaux, 'muaux) mformula" where
   "minit0 n (Formula.Neg \<phi>) = (if fv \<phi> = {} then MNeg (minit0 n \<phi>) else MRel empty_table)"
@@ -908,7 +919,7 @@ function (in maux) (sequential) minit0 :: "nat \<Rightarrow> Formula.formula \<R
     let mneg = map (minit0 n) (map remove_neg neg) in
     let vpos = map fv pos in
     let vneg = map fv neg in
-    MAnds vpos vneg (mpos @ mneg) (replicate (length l) []))"
+    MAnds vpos vneg (mpos @ mneg) (replicate (length l) mbuf_t_empty))"
 | "minit0 n (Formula.Exists \<phi>) = MExists (minit0 (Suc n) \<phi>)"
 | "minit0 n (Formula.Agg y \<omega> b f \<phi>) = MAgg (fv \<phi> \<subseteq> {0..<b}) y \<omega> b f (minit0 (b + n) \<phi>)"
 | "minit0 n (Formula.Prev I \<phi>) = MPrev I (minit0 n \<phi>) True [] []"
@@ -925,10 +936,10 @@ function (in maux) (sequential) minit0 :: "nat \<Rightarrow> Formula.formula \<R
     | _ \<Rightarrow> undefined))"
 | "minit0 n (Formula.MatchP I r) =
     (let (mr, \<phi>s) = to_mregex r
-    in MMatchP I mr (sorted_list_of_set (RPDs mr)) (map (minit0 n) \<phi>s) (replicate (length \<phi>s) []) [] [])"
+    in MMatchP I mr (sorted_list_of_set (RPDs mr)) (map (minit0 n) \<phi>s) (replicate (length \<phi>s) mbuf_t_empty) [] [])"
 | "minit0 n (Formula.MatchF I r) =
     (let (mr, \<phi>s) = to_mregex r
-    in MMatchF I mr (sorted_list_of_set (LPDs mr)) (map (minit0 n) \<phi>s) (replicate (length \<phi>s) []) [] 0 [])"
+    in MMatchF I mr (sorted_list_of_set (LPDs mr)) (map (minit0 n) \<phi>s) (replicate (length \<phi>s) mbuf_t_empty) [] 0 [])"
 | "minit0 n _ = undefined"
   by pat_completeness auto
 termination (in maux)
@@ -953,12 +964,34 @@ fun mbuf2_add :: "event_data table list \<Rightarrow> event_data table list \<Ri
   "mbuf2_add xs' ys' (xs, ys) = (xs @@ xs', ys @@ ys')"
 
 fun mbuf2S_add :: "event_data table list \<Rightarrow> event_data table list \<Rightarrow> ts list \<Rightarrow> event_data mbuf2S \<Rightarrow> event_data mbuf2S" where
-  "mbuf2S_add xs' ys' ts' (xs, ys, ts, skew) = (xs @ xs', ys @ ys', ts @ ts', skew)"
+  "mbuf2S_add xs' ys' ts' (xs, ys, ts, skew) = (xs @@ xs', ys @@ ys', ts @@ ts', skew)"
 
 fun mbuf2_take :: "(event_data table \<Rightarrow> event_data table \<Rightarrow> 'b) \<Rightarrow> event_data mbuf2 \<Rightarrow> 'b list \<times> event_data mbuf2" where
   "mbuf2_take f (xs, ys) = (case mbuf_t_cases xs of (None, xs') \<Rightarrow> ([], (xs', ys)) | (Some x, xs') \<Rightarrow>
     (case mbuf_t_cases ys of (None, ys') \<Rightarrow> ([], (x ## xs', ys')) | (Some y, ys') \<Rightarrow>
     let (zs, buf) = mbuf2_take f (xs', ys') in (f x y # zs, buf)))"
+
+fun mbuf2_list_take :: "(event_data table \<Rightarrow> event_data table \<Rightarrow> 'b) \<Rightarrow> event_data table list \<times> event_data table list \<Rightarrow> 'b list \<times> event_data table list \<times> event_data table list " where
+  "mbuf2_list_take f (x # xs, y # ys) = (let (zs, buf) = mbuf2_list_take f (xs, ys) in (f x y # zs, buf))"
+| "mbuf2_list_take f (xs, ys) = ([], (xs, ys))"
+
+lemma Rep_mbuf2_take_aux: "mbuf2_take f (xs, ys) = (zs, (xs', ys')) \<Longrightarrow>
+  mbuf2_list_take f (Rep_mbuf_t xs, Rep_mbuf_t ys) = (zs, (Rep_mbuf_t xs', Rep_mbuf_t ys'))"
+proof (induction f "(xs, ys)" arbitrary: xs ys zs xs' ys' rule: mbuf2_take.induct)
+  case (1 f xs ys)
+  obtain x xs'' where xs_def: "mbuf_t_cases xs = (x, xs'')"
+    by fastforce
+  obtain y ys'' where ys_def: "mbuf_t_cases ys = (y, ys'')"
+    by fastforce
+  show ?case
+    using 1 xs_def ys_def
+    by (cases x; cases y) (auto simp: mbuf_t_Cons.rep_eq split: prod.splits)
+qed
+
+lemma Rep_mbuf2_take: "mbuf2_take f buf = (zs, buf') \<Longrightarrow>
+  mbuf2_list_take f (map_prod Rep_mbuf_t Rep_mbuf_t buf) = (zs, (map_prod Rep_mbuf_t Rep_mbuf_t buf'))"
+  using Rep_mbuf2_take_aux
+  by (cases buf; cases buf') fastforce
 
 fun mbuf2t_take :: "(event_data table \<Rightarrow> event_data table \<Rightarrow> ts \<Rightarrow> 'b \<Rightarrow> 'b) \<Rightarrow> 'b \<Rightarrow>
     event_data mbuf2 \<Rightarrow> ts list \<Rightarrow> 'b \<times> event_data mbuf2 \<times> ts list" where
@@ -967,22 +1000,81 @@ fun mbuf2t_take :: "(event_data table \<Rightarrow> event_data table \<Rightarro
     (case ts of [] \<Rightarrow> (z, (x ## xs', y ## ys'), ts) | t # ts' \<Rightarrow>
     mbuf2t_take f (f x y t z) (xs', ys') ts')))"
 
+fun mbuf2t_list_take :: "(event_data table \<Rightarrow> event_data table \<Rightarrow> ts \<Rightarrow> 'b \<Rightarrow> 'b) \<Rightarrow> 'b \<Rightarrow>
+    event_data table list \<times> event_data table list \<Rightarrow> ts list \<Rightarrow> 'b \<times> (event_data table list \<times> event_data table list) \<times> ts list" where
+  "mbuf2t_list_take f z (x # xs, y # ys) (t # ts) = mbuf2t_list_take f (f x y t z) (xs, ys) ts"
+| "mbuf2t_list_take f z (xs, ys) ts = (z, (xs, ys), ts)"
+
+lemma Rep_mbuf2t_take_aux: "mbuf2t_take f z (xs, ys) ts = (zs, (xs', ys'), nts') \<Longrightarrow>
+  mbuf2t_list_take f z (Rep_mbuf_t xs, Rep_mbuf_t ys) ts = (zs, (Rep_mbuf_t xs', Rep_mbuf_t ys'), nts')"
+proof (induction f z "(xs, ys)" ts arbitrary: xs ys zs xs' ys' rule: mbuf2t_take.induct)
+  case (1 f z xs ys ts)
+  obtain x xs'' where xs_def: "mbuf_t_cases xs = (x, xs'')"
+    by fastforce
+  obtain y ys'' where ys_def: "mbuf_t_cases ys = (y, ys'')"
+    by fastforce
+  show ?case
+    using 1 xs_def ys_def
+    by (cases x; cases y) (auto simp: mbuf_t_Cons.rep_eq split: prod.splits list.splits)
+qed
+
+lemma Rep_mbuf2t_take: "mbuf2t_take f z buf ts = (zs, buf',  nts') \<Longrightarrow>
+  mbuf2t_list_take f z (map_prod Rep_mbuf_t Rep_mbuf_t buf) ts = (zs, (map_prod Rep_mbuf_t Rep_mbuf_t buf'), nts')"
+  using Rep_mbuf2t_take_aux
+  by (cases buf; cases buf') fastforce
+
 context maux begin
 context fixes args :: args begin
 
-fun eval_since :: "event_data table list \<Rightarrow> event_data mbuf2S \<Rightarrow> 'msaux \<Rightarrow>
-    event_data table list \<times> event_data mbuf2S \<times> 'msaux" where
-  "eval_since rs (x # xs, [], t # ts, skew) aux =
+fun eval_list_since :: "event_data table list \<Rightarrow> event_data table list \<times> event_data table list \<times> ts list \<times> bool \<Rightarrow> 'msaux \<Rightarrow>
+    event_data table list \<times> (event_data table list \<times> event_data table list \<times> ts list \<times> bool) \<times> 'msaux" where
+  "eval_list_since rs (x # xs, [], t # ts, skew) aux =
     (if skew \<or> memL (args_ivl args) 0
     then (rev rs, (x # xs, [], t # ts, skew), aux)
     else (let aux' = join_msaux args x (add_new_ts_msaux args t aux)
       in (rev (result_msaux args aux' # rs), (xs, [], ts, True), aux')))"
-| "eval_since rs (xs, y # ys, ts, True) aux =
-    eval_since rs (xs, ys, ts, False) (add_new_table_msaux args y aux)"
-| "eval_since rs (x # xs, y # ys, t # ts, False) aux =
+| "eval_list_since rs (xs, y # ys, ts, True) aux =
+    eval_list_since rs (xs, ys, ts, False) (add_new_table_msaux args y aux)"
+| "eval_list_since rs (x # xs, y # ys, t # ts, False) aux =
     (let aux' = add_new_table_msaux args y (join_msaux args x (add_new_ts_msaux args t aux))
-    in eval_since (result_msaux args aux' # rs) (xs, ys, ts, False) aux')"
-| "eval_since rs buf aux = (rev rs, buf, aux)"
+    in eval_list_since (result_msaux args aux' # rs) (xs, ys, ts, False) aux')"
+| "eval_list_since rs buf aux = (rev rs, buf, aux)"
+
+fun eval_since :: "event_data table list \<Rightarrow> event_data mbuf2S \<Rightarrow> 'msaux \<Rightarrow>
+    event_data table list \<times> event_data mbuf2S \<times> 'msaux" where
+  "eval_since rs (xs, ys, ts, skew) aux =
+    (case mbuf_t_cases ys of (None, ys') \<Rightarrow>
+      (case mbuf_t_cases xs of (Some x, xs') \<Rightarrow>
+        (case mbuf_t_cases ts of (Some t, ts') \<Rightarrow>
+    (if skew \<or> memL (args_ivl args) 0
+    then (rev rs, (x ## xs', mbuf_t_empty, t ## ts', skew), aux)
+    else (let aux' = join_msaux args x (add_new_ts_msaux args t aux)
+      in (rev (result_msaux args aux' # rs), (xs', mbuf_t_empty, ts', True), aux')))
+        | (None, ts') \<Rightarrow> (rev rs, (x ## xs', mbuf_t_empty, mbuf_t_empty, skew), aux))
+      | (None, xs') \<Rightarrow> (rev rs, (mbuf_t_empty, mbuf_t_empty, ts, skew), aux))
+    | (Some y, ys') \<Rightarrow>
+      if skew then eval_since rs (xs, ys', ts, False) (add_new_table_msaux args y aux) else
+      (case mbuf_t_cases xs of (Some x, xs') \<Rightarrow>
+        (case mbuf_t_cases ts of (Some t, ts') \<Rightarrow>
+    (let aux' = add_new_table_msaux args y (join_msaux args x (add_new_ts_msaux args t aux))
+    in eval_since (result_msaux args aux' # rs) (xs', ys', ts', False) aux')
+        | (None, ts') \<Rightarrow> (rev rs, (x ## xs', y ## ys', ts', skew), aux))
+      | (None, xs') \<Rightarrow> (rev rs, (mbuf_t_empty, y ## ys', ts, skew), aux)))"
+
+lemma Rep_eval_since: "eval_since rs (xs, ys, ts, skew) aux = (res, (xs', ys', ts', skew'), aux') \<Longrightarrow>
+  eval_list_since rs (Rep_mbuf_t xs, Rep_mbuf_t ys, Rep_mbuf_t ts, skew) aux = (res, (Rep_mbuf_t xs', Rep_mbuf_t ys', Rep_mbuf_t ts', skew'), aux')"
+proof (induction rs "(xs, ys, ts, skew)" aux arbitrary: xs ys ts skew res xs' ys' ts' skew' aux' rule: eval_since.induct)
+  case (1 rs xs ys ts skew aux)
+  obtain x xs'' where xs_def: "mbuf_t_cases xs = (x, xs'')"
+    by fastforce
+  obtain y ys'' where ys_def: "mbuf_t_cases ys = (y, ys'')"
+    by fastforce
+  obtain t ts'' where ts_def: "mbuf_t_cases ts = (t, ts'')"
+    by fastforce
+  show ?case
+    using 1 xs_def ys_def ts_def
+    by (cases x; cases y; cases t) (auto simp: mbuf_t_empty.rep_eq mbuf_t_Cons.rep_eq Let_def split: if_splits)
+qed
 
 end (* fixes args *)
 end (* maux *)
@@ -997,20 +1089,22 @@ proof (induct xs)
 qed simp
 
 fun mbufn_add :: "event_data table list list \<Rightarrow> event_data mbufn \<Rightarrow> event_data mbufn" where
-  "mbufn_add xs' xs = List.map2 (@) xs xs'"
+  "mbufn_add xs' xs = List.map2 (@@) xs xs'"
 
 function mbufn_take :: "(event_data table list \<Rightarrow> 'b \<Rightarrow> 'b) \<Rightarrow> 'b \<Rightarrow> event_data mbufn \<Rightarrow> 'b \<times> event_data mbufn" where
-  "mbufn_take f z buf = (if buf = [] \<or> [] \<in> set buf then (z, buf)
-    else mbufn_take f (f (map hd buf) z) (map tl buf))"
+  "mbufn_take f z buf = (if buf = [] \<or> (\<exists>x \<in> set buf. mbuf_t_is_empty x) then (z, buf)
+    else mbufn_take f (f (map (the \<circ> fst \<circ> mbuf_t_cases) buf) z) (map (snd \<circ> mbuf_t_cases) buf))"
   by pat_completeness auto
-termination by (relation "measure (\<lambda>(_, _, buf). size_list length buf)")
-    (auto simp: comp_def Suc_le_eq size_list_length_diff1)
+termination
+  apply (relation "measure (\<lambda>(_, _, buf). size_list size buf)")
+   apply   (auto simp: comp_def Suc_le_eq size_list_length_diff1)
+  sorry
 
 fun mbufnt_take :: "(event_data table list \<Rightarrow> ts \<Rightarrow> 'b \<Rightarrow> 'b) \<Rightarrow>
     'b \<Rightarrow> event_data mbufn \<Rightarrow> ts list \<Rightarrow> 'b \<times> event_data mbufn \<times> ts list" where
   "mbufnt_take f z buf ts =
-    (if [] \<in> set buf \<or> ts = [] then (z, buf, ts)
-    else mbufnt_take f (f (map hd buf) (hd ts) z) (map tl buf) (tl ts))"
+    (if (\<exists>x \<in> set buf. mbuf_t_is_empty x) \<or> ts = [] then (z, buf, ts)
+    else mbufnt_take f (f (map (the \<circ> fst \<circ> mbuf_t_cases) buf) (hd ts) z) (map (snd \<circ> mbuf_t_cases) buf) (tl ts))"
 
 fun match :: "Formula.trm list \<Rightarrow> event_data tuple \<Rightarrow> (nat \<rightharpoonup> event_data) option" where
   "match [] [] = Some Map.empty"
@@ -3063,7 +3157,7 @@ lemma list_all3_refl [intro?]:
   by (simp add: list_all3_conv_all_nth)
 
 definition wf_mbufn :: "nat \<Rightarrow> nat list \<Rightarrow> (nat \<Rightarrow> event_data table \<Rightarrow> bool) list \<Rightarrow> event_data mbufn \<Rightarrow> bool" where
-  "wf_mbufn i js Ps buf \<longleftrightarrow> list_all3 (\<lambda>P j xs. i \<le> j \<and> list_all2 P [i..<j] xs) Ps js buf"
+  "wf_mbufn i js Ps buf \<longleftrightarrow> list_all3 (\<lambda>P j xs. i \<le> j \<and> list_all2 P [i..<j] (Rep_mbuf_t xs)) Ps js buf"
 
 definition wf_mbuf2' :: "Formula.trace \<Rightarrow> _ \<Rightarrow> _ \<Rightarrow> nat \<Rightarrow> nat \<Rightarrow> event_data list set \<Rightarrow>
   Formula.formula \<Rightarrow> Formula.formula \<Rightarrow> event_data mbuf2 \<Rightarrow> bool" where
@@ -3097,10 +3191,10 @@ fun wf_mbuf2S :: "Formula.trace \<Rightarrow> _ \<Rightarrow> _ \<Rightarrow> na
   Formula.formula \<Rightarrow> \<I> \<Rightarrow> Formula.formula \<Rightarrow> event_data mbuf2S \<Rightarrow> nat \<Rightarrow> nat \<Rightarrow> bool" where
   "wf_mbuf2S \<sigma> P V j n R \<phi> I \<psi> (buf\<phi>, buf\<psi>, ts, skew) pIn pOut \<longleftrightarrow>
     list_all2 (\<lambda>i. qtable n (Formula.fv \<phi>) (mem_restr R) (\<lambda>v. Formula.sat \<sigma> V (map the v) i \<phi>))
-      [pOut ..< progress \<sigma> P \<phi> j] buf\<phi> \<and>
+      [pOut ..< progress \<sigma> P \<phi> j] (Rep_mbuf_t buf\<phi>) \<and>
     list_all2 (\<lambda>i. qtable n (Formula.fv \<psi>) (mem_restr R) (\<lambda>v. Formula.sat \<sigma> V (map the v) i \<psi>))
-      [pIn ..< progress \<sigma> P \<psi> j] buf\<psi> \<and>
-    list_all2 (\<lambda>i t. t = \<tau> \<sigma> i) [pOut ..< j] ts \<and>
+      [pIn ..< progress \<sigma> P \<psi> j] (Rep_mbuf_t buf\<psi>) \<and>
+    list_all2 (\<lambda>i t. t = \<tau> \<sigma> i) [pOut ..< j] (Rep_mbuf_t ts) \<and>
     pOut = (if skew then Suc pIn else pIn)"
 
 definition "sat_since_point pos \<sigma> V \<phi> \<psi> pIn i t x \<longleftrightarrow>
@@ -3803,9 +3897,9 @@ lemma wf_mbuf2'_0: "pred_mapping (\<lambda>x. x = 0) P \<Longrightarrow> wf_mbuf
   unfolding wf_mbuf2'_def wf_mbuf2_def
   by transfer simp
 
-lemma wf_mbufn'_0: "to_mregex r = (mr, \<phi>s) \<Longrightarrow> pred_mapping (\<lambda>x. x = 0) P \<Longrightarrow> wf_mbufn' \<sigma> P V 0 n R r (replicate (length \<phi>s) [])"
+lemma wf_mbufn'_0: "to_mregex r = (mr, \<phi>s) \<Longrightarrow> pred_mapping (\<lambda>x. x = 0) P \<Longrightarrow> wf_mbufn' \<sigma> P V 0 n R r (replicate (length \<phi>s) mbuf_t_empty)"
   unfolding wf_mbufn'_def wf_mbufn_def map_replicate_const[symmetric]
-  by (auto simp: list_all3_map intro: list_all3_refl simp: Min_eq_iff progress_regex_def)
+  by (auto simp: list_all3_map mbuf_t_empty.rep_eq intro: list_all3_refl simp: Min_eq_iff progress_regex_def)
 
 lemma wf_ts_0: "wf_ts \<sigma> P 0 \<phi> \<psi> []"
   unfolding wf_ts_def by simp
@@ -3908,7 +4002,7 @@ next
     by (cases l) (auto simp: Min_eq_iff)
   ultimately show ?case using Ands.hyps Ands.prems(2)
     by (auto simp: wf_mbufn_def list_all3_map list.rel_map map_replicate_const[symmetric] subset_eq
-        map_map[symmetric] map_append[symmetric] simp del: map_map map_append
+        map_map[symmetric] map_append[symmetric] mbuf_t_empty.rep_eq simp del: map_map map_append
         intro!: wf_mformula.Ands list_all2_appendI)
 next
   case (Neg \<phi>)
@@ -3933,12 +4027,12 @@ next
   case (Since \<phi> I \<psi>)
   then show ?case
     using wf_since_aux_Nil
-    by (auto simp add: init_args_def intro!: wf_mformula.Since wf_mbuf2'_0 wf_ts_0)
+    by (auto simp add: init_args_def mbuf_t_empty.rep_eq intro!: wf_mformula.Since wf_mbuf2'_0 wf_ts_0)
 next
   case (Not_Since \<phi> I \<psi>)
   then show ?case
     using wf_since_aux_Nil
-    by (auto simp add: init_args_def intro!: wf_mformula.Since wf_mbuf2'_0 wf_ts_0)
+    by (auto simp add: init_args_def mbuf_t_empty.rep_eq intro!: wf_mformula.Since wf_mbuf2'_0 wf_ts_0)
 next
   case (Until \<phi> I \<psi>)
   then show ?case
@@ -4630,41 +4724,41 @@ proof -
   let ?pOut = "progress \<sigma> P (Sincep pos \<phi> I \<psi>) j"
   obtain buf\<phi> buf\<psi> ts skew where buf_eq: "buf = (buf\<phi>, buf\<psi>, ts, skew)"
     by (metis surj_pair)
-  then have result_eq: "mbuf2S_add xs ys ?nts buf = (buf\<phi> @ xs, buf\<psi> @ ys, ts @ ?nts, skew)"
+  then have result_eq: "mbuf2S_add xs ys ?nts buf = (buf\<phi> @@ xs, buf\<psi> @@ ys, ts @@ ?nts, skew)"
     by simp
   show ?thesis
-    unfolding result_eq wf_mbuf2S.simps
+    unfolding result_eq wf_mbuf2S.simps mbuf_t_append.rep_eq
   proof (intro conjI)
     show "list_all2 (\<lambda>i. qtable n (fv \<phi>) (mem_restr R) (\<lambda>v. Formula.sat \<sigma> V (map the v) i \<phi>))
-        [?pOut..<progress \<sigma> P' \<phi> (j + \<delta>)] (buf\<phi> @ xs)" (is "?P [?pOut..<?p\<phi>'] (buf\<phi> @ xs)")
-      unfolding list_all2_append2
+        [?pOut..<progress \<sigma> P' \<phi> (j + \<delta>)] (Rep_mbuf_t buf\<phi> @ xs)" (is "?P [?pOut..<?p\<phi>'] (Rep_mbuf_t buf\<phi> @ xs)")
+      unfolding mbuf_t_append.rep_eq list_all2_append2
     proof (intro exI)
       let ?p\<phi> = "progress \<sigma> P \<phi> j"
       show "[?pOut..<?p\<phi>'] = [?pOut..<?p\<phi>] @ [?p\<phi>..<?p\<phi>'] \<and>
-          length [?pOut..<?p\<phi>] = length buf\<phi> \<and> length [?p\<phi>..<?p\<phi>'] = length xs \<and>
-          ?P [?pOut..<?p\<phi>] buf\<phi> \<and> ?P [?p\<phi>..<?p\<phi>'] xs"
+          length [?pOut..<?p\<phi>] = length (Rep_mbuf_t buf\<phi>) \<and> length [?p\<phi>..<?p\<phi>'] = length xs \<and>
+          ?P [?pOut..<?p\<phi>] (Rep_mbuf_t buf\<phi>) \<and> ?P [?p\<phi>..<?p\<phi>'] xs"
         using wf xs by (auto simp: buf_eq progress_Sincep upt_add_eq_append' progress_mono_gen[OF _ bounded rm]
             dest: list_all2_lengthD)
     qed
     show "list_all2 (\<lambda>i. qtable n (fv \<psi>) (mem_restr R) (\<lambda>v. Formula.sat \<sigma> V (map the v) i \<psi>))
-        [?pIn..<progress \<sigma> P' \<psi> (j + \<delta>)] (buf\<psi> @ ys)" (is "?P [?pIn..<?p\<psi>'] (buf\<psi> @ ys)")
+        [?pIn..<progress \<sigma> P' \<psi> (j + \<delta>)] (Rep_mbuf_t buf\<psi> @ ys)" (is "?P [?pIn..<?p\<psi>'] (Rep_mbuf_t buf\<psi> @ ys)")
       unfolding list_all2_append2
     proof (intro exI)
       let ?p\<psi> = "progress \<sigma> P \<psi> j"
       show "[?pIn..<?p\<psi>'] = [?pIn..<?p\<psi>] @ [?p\<psi>..<?p\<psi>'] \<and>
-          length [?pIn..<?p\<psi>] = length buf\<psi> \<and> length [?p\<psi>..<?p\<psi>'] = length ys \<and>
-          ?P [?pIn..<?p\<psi>] buf\<psi> \<and> ?P [?p\<psi>..<?p\<psi>'] ys"
+          length [?pIn..<?p\<psi>] = length (Rep_mbuf_t buf\<psi>) \<and> length [?p\<psi>..<?p\<psi>'] = length ys \<and>
+          ?P [?pIn..<?p\<psi>] (Rep_mbuf_t buf\<psi>) \<and> ?P [?p\<psi>..<?p\<psi>'] ys"
         using wf ys by (auto simp: buf_eq progress_Sincep upt_add_eq_append' progress_mono_gen[OF _ bounded rm]
             dest: list_all2_lengthD)
     qed
-    show "list_all2 (\<lambda>i t. t = \<tau> \<sigma> i) [?pOut..<j + \<delta>] (ts @ ?nts)"
+    show "list_all2 (\<lambda>i t. t = \<tau> \<sigma> i) [?pOut..<j + \<delta>] (Rep_mbuf_t ts @ ?nts)"
       unfolding list_all2_append2
     proof (intro exI)
       have "?pOut \<le> j"
         by (rule progress_le_gen[OF bounded(1)])
       then show "[?pOut..<j + \<delta>] = [?pOut..<j] @ [j..<j + \<delta>] \<and>
-          length [?pOut..<j] = length ts \<and> length [j..<j + \<delta>] = length ?nts \<and>
-          list_all2 (\<lambda>i t. t = \<tau> \<sigma> i) [?pOut..<j] ts \<and> list_all2 (\<lambda>i t. t = \<tau> \<sigma> i) [j..<j + \<delta>] ?nts"
+          length [?pOut..<j] = length (Rep_mbuf_t ts) \<and> length [j..<j + \<delta>] = length ?nts \<and>
+          list_all2 (\<lambda>i t. t = \<tau> \<sigma> i) [?pOut..<j] (Rep_mbuf_t ts) \<and> list_all2 (\<lambda>i t. t = \<tau> \<sigma> i) [j..<j + \<delta>] ?nts"
         using wf by (auto simp add: buf_eq list.rel_map list.rel_refl simp flip: upt_add_eq_append'
               dest: list_all2_lengthD)
     qed
@@ -4871,16 +4965,30 @@ lemma (in msaux) wf_since_aux_result:
     done
   done
 
-lemma (in maux) eval_since_gen:
+fun Rep_wf_mbuf2S :: "Formula.trace \<Rightarrow> _ \<Rightarrow> _ \<Rightarrow> nat \<Rightarrow> nat \<Rightarrow> event_data list set \<Rightarrow>
+  Formula.formula \<Rightarrow> \<I> \<Rightarrow> Formula.formula \<Rightarrow> event_data table list \<times> event_data table list \<times> ts list \<times> bool \<Rightarrow> nat \<Rightarrow> nat \<Rightarrow> bool" where
+  "Rep_wf_mbuf2S \<sigma> P V j n R \<phi> I \<psi> (buf\<phi>, buf\<psi>, ts, skew) pIn pOut \<longleftrightarrow>
+    list_all2 (\<lambda>i. qtable n (Formula.fv \<phi>) (mem_restr R) (\<lambda>v. Formula.sat \<sigma> V (map the v) i \<phi>))
+      [pOut ..< progress \<sigma> P \<phi> j] buf\<phi> \<and>
+    list_all2 (\<lambda>i. qtable n (Formula.fv \<psi>) (mem_restr R) (\<lambda>v. Formula.sat \<sigma> V (map the v) i \<psi>))
+      [pIn ..< progress \<sigma> P \<psi> j] buf\<psi> \<and>
+    list_all2 (\<lambda>i t. t = \<tau> \<sigma> i) [pOut ..< j] ts \<and>
+    pOut = (if skew then Suc pIn else pIn)"
+
+lemma Rep_wf_mbuf2S: "Rep_wf_mbuf2S \<sigma> P V j n R \<phi> I \<psi> (Rep_mbuf_t buf\<phi>, Rep_mbuf_t buf\<psi>, Rep_mbuf_t ts, skew) pIn pOut \<longleftrightarrow>
+  wf_mbuf2S \<sigma> P V j n R \<phi> I \<psi> (buf\<phi>, buf\<psi>, ts, skew) pIn pOut"
+  by auto
+
+lemma (in maux) eval_since_list_gen:
   assumes pre:
       "list_all2 (\<lambda>i. qtable n (Formula.fv \<psi>) (mem_restr R) (\<lambda>v. Formula.sat \<sigma> V (map the v) i (Sincep pos \<phi> I \<psi>)))
         [start..<pOut] (rev zs)" (is "?A pOut (rev zs)")
-      "wf_mbuf2S \<sigma> P V j n R \<phi> I \<psi> buf pIn pOut" (is "?B buf pIn pOut")
+      "Rep_wf_mbuf2S \<sigma> P V j n R \<phi> I \<psi> buf pIn pOut" (is "?B buf pIn pOut")
       "wf_since_aux \<sigma> V R args \<phi> \<psi> aux pIn pOut" (is "?C aux pIn pOut")
       "pIn \<le> progress \<sigma> P \<phi> j" "pIn \<le> progress \<sigma> P \<psi> j"
       "pOut \<le> progress \<sigma> P (Sincep pos \<phi> I \<psi>) j"
       "start \<le> pOut"
-      "(zs', buf', aux') = eval_since args zs buf aux"
+      "(zs', buf', aux') = eval_list_since args zs buf aux"
     and bounded: "pred_mapping (\<lambda>x. x \<le> j) P"
     and fvi_subset: "fv \<phi> \<subseteq> fv \<psi>"
     and args_ivl: "args_ivl args = I"
@@ -4893,7 +5001,7 @@ lemma (in maux) eval_since_gen:
       ?B buf' (min (progress \<sigma> P \<phi> j) (progress \<sigma> P \<psi> j)) (progress \<sigma> P (Sincep pos \<phi> I \<psi>) j) \<and>
       ?C aux' (min (progress \<sigma> P \<phi> j) (progress \<sigma> P \<psi> j)) (progress \<sigma> P (Sincep pos \<phi> I \<psi>) j)"
   using pre
-proof (induction zs buf aux arbitrary: pIn pOut zs' buf' aux' taking: args rule: eval_since.induct)
+proof (induction zs buf aux arbitrary: pIn pOut zs' buf' aux' taking: args rule: eval_list_since.induct)
   case (1 zs x xs t ts skew aux)
   note wf_result = "1.prems"(1)
   note wf_buf = "1.prems"(2)
@@ -4901,7 +5009,8 @@ proof (induction zs buf aux arbitrary: pIn pOut zs' buf' aux' taking: args rule:
   note leqs = "1.prems"(4-7)
   note result_eq = "1.prems"(8)
   have pIn_eq: "pIn = progress \<sigma> P \<psi> j" and \<psi>_before_\<phi>: "progress \<sigma> P \<psi> j \<le> progress \<sigma> P \<phi> j"
-    using wf_buf leqs by (auto dest: list_all2_lengthD)
+    using wf_buf leqs
+    by (auto dest: list_all2_lengthD split: if_splits)
   show ?case proof (cases "skew \<or> memL (args_ivl args) 0")
     case True
     then have eqs: "zs' = rev zs" "buf' = (x # xs, [], t # ts, skew)" "aux' = aux"
@@ -4949,7 +5058,7 @@ next
   note result_eq = "2.prems"(8)
   let ?arg_aux = "add_new_table_msaux args y aux"
   show ?case proof (rule "2.IH")
-    show "(zs', buf', aux') = eval_since args zs (xs, ys, ts, False) ?arg_aux"
+    show "(zs', buf', aux') = eval_list_since args zs (xs, ys, ts, False) ?arg_aux"
       using result_eq by (simp add: Let_def)
     show "?A pOut (rev zs)" by fact
     show "?B (xs, ys, ts, False) (Suc pIn) pOut"
@@ -4995,7 +5104,7 @@ next
     ultimately show "Suc pOut \<le> progress \<sigma> P (Sincep pos \<phi> I \<psi>) j"
       using wf_buf by (simp add: progress_Sincep)
     show "start \<le> Suc pOut" using leqs by simp
-    show "(zs', buf', aux') = eval_since args (result_msaux args ?arg_aux # zs)
+    show "(zs', buf', aux') = eval_list_since args (result_msaux args ?arg_aux # zs)
          (xs, ys, ts, False) ?arg_aux"
       using result_eq by (simp add: Let_def)
   qed
@@ -5023,7 +5132,7 @@ next
     apply (simp add: progress_Sincep)
     by (smt (z3) calculation list.rel_distinct(1) min_def upt_eq_Nil_conv)
   ultimately show ?case
-    using "4_4" by (simp only: eval_since.simps prod.inject)
+    using "4_4" by (simp only: eval_list_since.simps prod.inject)
 next
   case ("4_5" zs v ve aux)
   then have "pIn = min (progress \<sigma> P \<phi> j) (progress \<sigma> P \<psi> j)"
@@ -5033,7 +5142,7 @@ next
     apply (simp add: progress_Sincep)
     by (smt (z3) bot_nat_0.extremum_uniqueI bounded dual_order.trans min.commute min_def pred_mapping_mono_strong progress_le_gen)
   ultimately show ?case
-    using "4_5" by (simp only: eval_since.simps prod.inject)
+    using "4_5" by (simp only: eval_list_since.simps prod.inject)
 next
   case ("4_6" zs v vb aux)
   then have "pIn = min (progress \<sigma> P \<phi> j) (progress \<sigma> P \<psi> j)"
@@ -5044,7 +5153,37 @@ next
     apply (simp add: progress_Sincep)
     by (smt (z3) bot_nat_0.extremum_uniqueI bounded dual_order.trans min.commute min_def pred_mapping_mono_strong progress_le_gen)
   ultimately show ?case
-    using "4_6" by (simp only: eval_since.simps prod.inject)
+    using "4_6" by (simp only: eval_list_since.simps prod.inject)
+qed
+
+lemma (in maux) eval_since_gen:
+  assumes pre:
+      "list_all2 (\<lambda>i. qtable n (Formula.fv \<psi>) (mem_restr R) (\<lambda>v. Formula.sat \<sigma> V (map the v) i (Sincep pos \<phi> I \<psi>)))
+        [start..<pOut] (rev zs)" (is "?A pOut (rev zs)")
+      "wf_mbuf2S \<sigma> P V j n R \<phi> I \<psi> buf pIn pOut" (is "?B buf pIn pOut")
+      "wf_since_aux \<sigma> V R args \<phi> \<psi> aux pIn pOut" (is "?C aux pIn pOut")
+      "pIn \<le> progress \<sigma> P \<phi> j" "pIn \<le> progress \<sigma> P \<psi> j"
+      "pOut \<le> progress \<sigma> P (Sincep pos \<phi> I \<psi>) j"
+      "start \<le> pOut"
+      "(zs', buf', aux') = eval_since args zs buf aux"
+    and bounded: "pred_mapping (\<lambda>x. x \<le> j) P"
+    and fvi_subset: "fv \<phi> \<subseteq> fv \<psi>"
+    and args_ivl: "args_ivl args = I"
+    and args_n: "args_n args = n"
+    and args_L: "args_L args = Formula.fv \<phi>"
+    and args_R: "args_R args = Formula.fv \<psi>"
+    and args_pos: "args_pos args = pos"
+  shows
+      "?A (progress \<sigma> P (Sincep pos \<phi> I \<psi>) j) zs' \<and>
+      ?B buf' (min (progress \<sigma> P \<phi> j) (progress \<sigma> P \<psi> j)) (progress \<sigma> P (Sincep pos \<phi> I \<psi>) j) \<and>
+      ?C aux' (min (progress \<sigma> P \<phi> j) (progress \<sigma> P \<psi> j)) (progress \<sigma> P (Sincep pos \<phi> I \<psi>) j)"
+proof -
+  obtain xs ys ts skew where buf_def: "buf = (xs, ys, ts, skew)"
+    by (cases buf) auto
+  obtain xs' ys' ts' skew' where buf'_def: "buf' = (xs', ys', ts', skew')"
+    by (cases buf') auto
+  show ?thesis
+    by (rule eval_since_list_gen[OF assms(1) assms(2)[unfolded buf_def, folded Rep_wf_mbuf2S] assms(3-7) Rep_eval_since[OF pre(8)[unfolded buf_def buf'_def, symmetric], symmetric] assms(9-), unfolded Rep_wf_mbuf2S, folded buf'_def])
 qed
 
 lemma (in maux) eval_since:
@@ -5903,62 +6042,56 @@ lemma wf_mbuf2_add:
         exI[where x="[i..<jb]"] exI[where x="[jb..<jb']"] split: prod.splits)
   done
 
+definition Rep_wf_mbufn :: "nat \<Rightarrow> nat list \<Rightarrow> (nat \<Rightarrow> event_data table \<Rightarrow> bool) list \<Rightarrow> event_data table list list \<Rightarrow> bool" where
+  "Rep_wf_mbufn i js Ps buf \<longleftrightarrow> list_all3 (\<lambda>P j xs. i \<le> j \<and> list_all2 P [i..<j] xs) Ps js buf"
+
+lemma Rep_wf_mbufn: "Rep_wf_mbufn i js Ps (map Rep_mbuf_t buf) \<longleftrightarrow> wf_mbufn i js Ps buf"
+  by (auto simp: Rep_wf_mbufn_def wf_mbufn_def list_all3_conv_all_nth)
+
+fun Rep_mbufn_add :: "event_data table list list \<Rightarrow> event_data table list list \<Rightarrow> event_data table list list" where
+  "Rep_mbufn_add xs' xs = List.map2 (@) xs xs'"
+
+lemma Rep_mbufn_add: "Rep_mbufn_add xss (map Rep_mbuf_t buf) = map Rep_mbuf_t (mbufn_add xss buf)"
+  by (auto simp: comp_def zip_map1 mbuf_t_append.rep_eq)
+
+lemma Rep_wf_mbufn_add:
+  assumes "Rep_wf_mbufn i js Ps buf"
+    and "list_all3 list_all2 Ps (List.map2 (\<lambda>j j'. [j..<j']) js js') xss"
+    and "list_all2 (\<le>) js js'"
+  shows "Rep_wf_mbufn i js' Ps (Rep_mbufn_add xss buf)"
+  unfolding Rep_wf_mbufn_def list_all3_conv_all_nth
+proof safe
+  show "length Ps = length js'" "length js' = length (Rep_mbufn_add xss buf)"
+    using assms unfolding Rep_wf_mbufn_def list_all3_conv_all_nth list_all2_conv_all_nth by auto
+next
+  fix k assume k: "k < length Ps"
+  then show "i \<le> js' ! k"
+    using assms unfolding Rep_wf_mbufn_def list_all3_conv_all_nth list_all2_conv_all_nth
+    by (auto 0 4 dest: spec[of _ i])
+  from k have " [i..<js' ! k] =  [i..<js ! k] @ [js ! k ..<js' ! k]" and
+    "length [i..<js ! k] = length (buf ! k)"
+    using assms(1,3) unfolding Rep_wf_mbufn_def list_all3_conv_all_nth list_all2_conv_all_nth
+    by (auto simp: upt_append)
+  with k show "list_all2 (Ps ! k) [i..<js' ! k] (Rep_mbufn_add xss buf ! k)"
+    using assms[unfolded Rep_wf_mbufn_def list_all3_conv_all_nth]
+    by (auto simp add: list_all2_append)
+qed
+
 lemma wf_mbufn_add:
   assumes "wf_mbufn i js Ps buf"
     and "list_all3 list_all2 Ps (List.map2 (\<lambda>j j'. [j..<j']) js js') xss"
     and "list_all2 (\<le>) js js'"
   shows "wf_mbufn i js' Ps (mbufn_add xss buf)"
-  unfolding wf_mbufn_def list_all3_conv_all_nth
-proof safe
-  show "length Ps = length js'" "length js' = length (mbufn_add xss buf)"
-    using assms unfolding wf_mbufn_def list_all3_conv_all_nth list_all2_conv_all_nth by auto
-next
-  fix k assume k: "k < length Ps"
-  then show "i \<le> js' ! k"
-    using assms unfolding wf_mbufn_def list_all3_conv_all_nth list_all2_conv_all_nth
-    by (auto 0 4 dest: spec[of _ i])
-  from k have " [i..<js' ! k] =  [i..<js ! k] @ [js ! k ..<js' ! k]" and
-    "length [i..<js ! k] = length (buf ! k)"
-    using assms(1,3) unfolding wf_mbufn_def list_all3_conv_all_nth list_all2_conv_all_nth
-    by (auto simp: upt_append)
-  with k show "list_all2 (Ps ! k) [i..<js' ! k] (mbufn_add xss buf ! k)"
-    using assms[unfolded wf_mbufn_def list_all3_conv_all_nth]
-    by (auto simp add: list_all2_append)
-qed
-
-fun mbuf2_list_take :: "(event_data table \<Rightarrow> event_data table \<Rightarrow> 'b) \<Rightarrow> event_data table list \<times> event_data table list \<Rightarrow> 'b list \<times> event_data table list \<times> event_data table list " where
-  "mbuf2_list_take f (x # xs, y # ys) = (let (zs, buf) = mbuf2_list_take f (xs, ys) in (f x y # zs, buf))"
-| "mbuf2_list_take f (xs, ys) = ([], (xs, ys))"
-
-lemma Rep_mbuf_t_cases[simp]:
-  "mbuf_t_cases xs = (None, xs') \<Longrightarrow> Rep_mbuf_t xs = []"
-  "mbuf_t_cases xs = (None, xs') \<Longrightarrow> Rep_mbuf_t xs' = []"
-  "mbuf_t_cases xs = (Some x, xs') \<Longrightarrow> Rep_mbuf_t xs = x # Rep_mbuf_t xs'"
-  subgoal by transfer (auto split: option.splits list.splits)
-  subgoal by transfer (auto split: option.splits list.splits)
-  subgoal by transfer (auto split: option.splits list.splits)
-  done
-
-lemma Rep_mbuf2_take: "mbuf2_take f (xs, ys) = (zs, (xs', ys')) \<Longrightarrow>
-  mbuf2_list_take f (Rep_mbuf_t xs, Rep_mbuf_t ys) = (zs, (Rep_mbuf_t xs', Rep_mbuf_t ys'))"
-proof (induction f "(xs, ys)" arbitrary: xs ys zs xs' ys' rule: mbuf2_take.induct)
-  case (1 f xs ys)
-  obtain x xs'' where xs_def: "mbuf_t_cases xs = (x, xs'')"
-    by fastforce
-  obtain y ys'' where ys_def: "mbuf_t_cases ys = (y, ys'')"
-    by fastforce
-  show ?case
-    using 1 xs_def ys_def
-    by (cases x; cases y) (auto simp: mbuf_t_Cons.rep_eq split: prod.splits)
-qed
+  unfolding Rep_wf_mbufn[symmetric] Rep_mbufn_add[symmetric]
+  by (rule Rep_wf_mbufn_add[OF assms(1)[folded Rep_wf_mbufn] assms(2-)])
 
 definition Rep_wf_mbuf2 :: "nat \<Rightarrow> nat \<Rightarrow> nat \<Rightarrow> (nat \<Rightarrow> event_data table \<Rightarrow> bool) \<Rightarrow> (nat \<Rightarrow> event_data table \<Rightarrow> bool) \<Rightarrow>
     event_data table list \<times> event_data table list \<Rightarrow> bool" where
   "Rep_wf_mbuf2 i ja jb P Q buf \<longleftrightarrow> i \<le> ja \<and> i \<le> jb \<and> (case buf of (xs, ys) \<Rightarrow>
     list_all2 P [i..<ja] xs \<and> list_all2 Q [i..<jb] ys)"
 
-lemma Rep_wf_mbuf2: "Rep_wf_mbuf2 i ja jb P Q (Rep_mbuf_t xs, Rep_mbuf_t ys) \<longleftrightarrow>
-  wf_mbuf2 i ja jb P Q (xs, ys)"
+lemma Rep_wf_mbuf2: "Rep_wf_mbuf2 i ja jb P Q (map_prod Rep_mbuf_t Rep_mbuf_t buf) \<longleftrightarrow>
+  wf_mbuf2 i ja jb P Q buf"
   by (auto simp: Rep_wf_mbuf2_def wf_mbuf2_def)
 
 lemma mbuf2_list_take_eqD:
@@ -5975,15 +6108,8 @@ lemma mbuf2_take_eqD:
     and "wf_mbuf2 i ja jb P Q buf"
   shows "wf_mbuf2 (min ja jb) ja jb P Q buf'"
     and "list_all2 (\<lambda>i z. \<exists>x y. P i x \<and> Q i y \<and> z = f x y) [i..<min ja jb] zs"
-proof -
-  obtain xs ys where buf_def: "buf = (xs, ys)"
-    by fastforce
-  obtain xs' ys' where buf'_def: "buf' = (xs', ys')"
-    by fastforce
-  show "wf_mbuf2 (min ja jb) ja jb P Q buf'" "list_all2 (\<lambda>i z. \<exists>x y. P i x \<and> Q i y \<and> z = f x y) [i..<min ja jb] zs"
-    using mbuf2_list_take_eqD[OF Rep_mbuf2_take[OF assms(1)[unfolded buf_def buf'_def]], OF assms(2)[unfolded buf_def, folded Rep_wf_mbuf2]]
-    by (auto simp: buf'_def Rep_wf_mbuf2[symmetric])
-qed
+  using mbuf2_list_take_eqD[OF Rep_mbuf2_take[OF assms(1)] assms(2)[folded Rep_wf_mbuf2]]
+  by (auto simp: Rep_wf_mbuf2[symmetric])
 
 lemma list_all3_Nil[simp]:
   "list_all3 P xs ys [] \<longleftrightarrow> xs = [] \<and> ys = []"
@@ -6006,51 +6132,55 @@ lemma list_all3_mono_strong: "list_all3 P xs ys zs \<Longrightarrow>
 definition Mini where
   "Mini i js = (if js = [] then i else Min (set js))"
 
-lemma wf_mbufn_in_set_Mini:
-  assumes "wf_mbufn i js Ps buf"
+lemma Rep_wf_mbufn_in_set_Mini:
+  assumes "Rep_wf_mbufn i js Ps buf"
   shows "[] \<in> set buf \<Longrightarrow> Mini i js = i"
   unfolding in_set_conv_nth
 proof (elim exE conjE)
   fix k
   have "i \<le> j" if "j \<in> set js" for j
-    using that assms unfolding wf_mbufn_def list_all3_conv_all_nth in_set_conv_nth by auto
+    using that assms unfolding Rep_wf_mbufn_def list_all3_conv_all_nth in_set_conv_nth by auto
   moreover assume "k < length buf" "buf ! k = []"
   ultimately show ?thesis using assms
-    unfolding Mini_def wf_mbufn_def list_all3_conv_all_nth
+    unfolding Mini_def Rep_wf_mbufn_def list_all3_conv_all_nth
     by (auto 0 4 dest!: spec[of _ k] intro: Min_eqI simp: in_set_conv_nth)
 qed
 
-lemma wf_mbufn_notin_set:
+lemma wf_mbufn_in_set_Mini:
   assumes "wf_mbufn i js Ps buf"
+  shows "(\<exists>x \<in> set buf. mbuf_t_is_empty x) \<Longrightarrow> Mini i js = i"
+  using Rep_wf_mbufn_in_set_Mini[OF assms[folded Rep_wf_mbufn]]
+  by transfer auto
+
+lemma Rep_wf_mbufn_notin_set:
+  assumes "Rep_wf_mbufn i js Ps buf"
   shows "[] \<notin> set buf \<Longrightarrow> j \<in> set js \<Longrightarrow> i < j"
-  using assms unfolding wf_mbufn_def list_all3_conv_all_nth
+  using assms unfolding Rep_wf_mbufn_def list_all3_conv_all_nth
   by (cases "i \<in> set js") (auto intro: le_neq_implies_less simp: in_set_conv_nth)
 
-lemma wf_mbufn_map_tl:
-  "wf_mbufn i js Ps buf \<Longrightarrow> [] \<notin> set buf \<Longrightarrow> wf_mbufn (Suc i) js Ps (map tl buf)"
-  by (auto simp: wf_mbufn_def list_all3_map Suc_le_eq
+lemma wf_mbufn_notin_set:
+  assumes "wf_mbufn i js Ps buf"
+  shows "\<not>(\<exists>x \<in> set buf. mbuf_t_is_empty x) \<Longrightarrow> j \<in> set js \<Longrightarrow> i < j"
+  using Rep_wf_mbufn_notin_set[OF assms[folded Rep_wf_mbufn]]
+  by transfer auto
+
+lemma Rep_wf_mbufn_map_tl:
+  "Rep_wf_mbufn i js Ps buf \<Longrightarrow> [] \<notin> set buf \<Longrightarrow> Rep_wf_mbufn (Suc i) js Ps (map tl buf)"
+  by (auto simp: Rep_wf_mbufn_def list_all3_map Suc_le_eq
       dest: rel_funD[OF tl_transfer]  elim!: list_all3_mono_strong le_neq_implies_less)
+
+lemma map_tl_aux: assumes "[] \<notin> set buf"
+  shows "map (\<lambda>x. snd (case x of [] \<Rightarrow> (None, x) | y # x \<Rightarrow> (Some y, x))) buf = map tl buf"
+  using assms
+  by (auto split: list.splits)
+
+lemma wf_mbufn_map_tl:
+  "wf_mbufn i js Ps buf \<Longrightarrow> \<not>(\<exists>x \<in> set buf. mbuf_t_is_empty x) \<Longrightarrow> wf_mbufn (Suc i) js Ps (map (snd \<circ> mbuf_t_cases) buf)"
+  unfolding Rep_wf_mbufn[symmetric]
+  by (drule Rep_wf_mbufn_map_tl; transfer) (auto simp: comp_def map_tl_aux)
 
 lemma list_all3_list_all2I: "list_all3 (\<lambda>x y z. Q x z) xs ys zs \<Longrightarrow> list_all2 Q xs zs"
   by (induct xs ys zs rule: list_all3.induct) auto
-
-fun mbuf2t_list_take :: "(event_data table \<Rightarrow> event_data table \<Rightarrow> ts \<Rightarrow> 'b \<Rightarrow> 'b) \<Rightarrow> 'b \<Rightarrow>
-    event_data table list \<times> event_data table list \<Rightarrow> ts list \<Rightarrow> 'b \<times> (event_data table list \<times> event_data table list) \<times> ts list" where
-  "mbuf2t_list_take f z (x # xs, y # ys) (t # ts) = mbuf2t_list_take f (f x y t z) (xs, ys) ts"
-| "mbuf2t_list_take f z (xs, ys) ts = (z, (xs, ys), ts)"
-
-lemma Rep_mbuf2t_take: "mbuf2t_take f z (xs, ys) ts = (zs, (xs', ys'), nts') \<Longrightarrow>
-  mbuf2t_list_take f z (Rep_mbuf_t xs, Rep_mbuf_t ys) ts = (zs, (Rep_mbuf_t xs', Rep_mbuf_t ys'), nts')"
-proof (induction f z "(xs, ys)" ts arbitrary: xs ys zs xs' ys' rule: mbuf2t_take.induct)
-  case (1 f z xs ys ts)
-  obtain x xs'' where xs_def: "mbuf_t_cases xs = (x, xs'')"
-    by fastforce
-  obtain y ys'' where ys_def: "mbuf_t_cases ys = (y, ys'')"
-    by fastforce
-  show ?case
-    using 1 xs_def ys_def
-    by (cases x; cases y) (auto simp: mbuf_t_Cons.rep_eq split: prod.splits list.splits)
-qed
 
 lemma mbuf2t_take_list_eqD:
   assumes "mbuf2t_list_take f z buf nts = (z', buf', nts')"
@@ -6081,12 +6211,25 @@ proof -
     by (auto simp: buf'_def Rep_wf_mbuf2[symmetric])
 qed
 
-lemma wf_mbufn_take:
-  assumes "mbufn_take f z buf = (z', buf')"
-    and "wf_mbufn i js Ps buf"
-  shows "wf_mbufn (Mini i js) js Ps buf'"
-  using assms unfolding wf_mbufn_def
-proof (induction f z buf arbitrary: i z' buf' rule: mbufn_take.induct)
+function Rep_mbufn_take :: "(event_data table list \<Rightarrow> 'b \<Rightarrow> 'b) \<Rightarrow> 'b \<Rightarrow> event_data table list list \<Rightarrow> 'b \<times> event_data table list list" where
+  "Rep_mbufn_take f z buf = (if buf = [] \<or> [] \<in> set buf then (z, buf)
+    else Rep_mbufn_take f (f (map hd buf) z) (map tl buf))"
+  by pat_completeness auto
+termination by (relation "measure (\<lambda>(_, _, buf). size_list length buf)")
+    (auto simp: comp_def Suc_le_eq size_list_length_diff1)
+
+lemma Rep_mbufn_take: "mbufn_take f z buf = (z', buf') \<Longrightarrow>
+  Rep_mbufn_take f z (map Rep_mbuf_t buf) = (z', map Rep_mbuf_t buf')"
+  apply (induction f z buf arbitrary: z' buf' rule: mbufn_take.induct)
+  apply (auto simp del: Rep_mbufn_take.simps mbufn_take.simps)
+  sorry
+
+lemma Rep_wf_mbufn_take:
+  assumes "Rep_mbufn_take f z buf = (z', buf')"
+    and "Rep_wf_mbufn i js Ps buf"
+  shows "Rep_wf_mbufn (Mini i js) js Ps buf'"
+  using assms unfolding Rep_wf_mbufn_def
+proof (induction f z buf arbitrary: i z' buf' rule: Rep_mbufn_take.induct)
   case rec: (1 f z buf)
   show ?case proof (cases "buf = []")
     case True
@@ -6114,12 +6257,60 @@ proof (induction f z buf arbitrary: i z' buf' rule: mbufn_take.induct)
         show "list_all3 (\<lambda>P j xs. Suc i \<le> j \<and> list_all2 P [Suc i..<j] xs) Ps js (map tl buf)"
           using False rec.prems(2)
           by (auto simp: list_all3_map elim!: list_all3_mono_strong dest: list.rel_sel[THEN iffD1])
-        show "mbufn_take f (f (map hd buf) z) (map tl buf) = (z', buf')"
+        show "Rep_mbufn_take f (f (map hd buf) z) (map tl buf) = (z', buf')"
           using nonempty False rec.prems(1) by simp
       qed
     qed
   qed
 qed
+
+lemma wf_mbufn_take:
+  assumes "mbufn_take f z buf = (z', buf')"
+    and "wf_mbufn i js Ps buf"
+  shows "wf_mbufn (Mini i js) js Ps buf'"
+  unfolding Rep_wf_mbufn[symmetric]
+  by (rule Rep_wf_mbufn_take[OF Rep_mbufn_take[OF assms(1)] assms(2)[folded Rep_wf_mbufn]])
+
+fun Rep_mbufnt_take :: "(event_data table list \<Rightarrow> ts \<Rightarrow> 'b \<Rightarrow> 'b) \<Rightarrow>
+     'b \<Rightarrow> event_data table list list \<Rightarrow> ts list \<Rightarrow> 'b \<times> event_data table list list \<times> ts list" where
+  "Rep_mbufnt_take f z buf ts =
+    (if [] \<in> set buf \<or> ts = [] then (z, buf, ts)
+    else Rep_mbufnt_take f (f (map hd buf) (hd ts) z) (map tl buf) (tl ts))"
+
+lemma Rep_mbufnt_take_eqD:
+  assumes "Rep_mbufnt_take f z buf nts = (z', buf', nts')"
+    and "Rep_wf_mbufn i js Ps buf"
+    and "list_all2 R [i..<j] nts"
+    and "\<And>k. k \<in> set js \<Longrightarrow> k \<le> j"
+    and "k = Mini (i + length nts) js"
+  shows "Rep_wf_mbufn k js Ps buf'"
+    and "list_all2 R [k..<j] nts'"
+  using assms(1-4) unfolding assms(5)
+proof (induction f z buf nts arbitrary: i z' buf' nts' rule: Rep_mbufnt_take.induct)
+  case IH: (1 f z buf nts)
+  note Rep_mbufnt_take.simps[simp del]
+  case 1
+  then have *: "list_all2 R [Suc i..<j] (tl nts)"
+    by (auto simp: list.rel_sel[of R "[i..<j]" nts, simplified])
+  from 1 show ?case
+    using Rep_wf_mbufn_in_set_Mini[OF 1(2)]
+    by (subst (asm) Rep_mbufnt_take.simps)
+      (force simp: Mini_def Rep_wf_mbufn_def split: if_splits prod.splits elim!: list_all3_mono_strong
+        dest!: IH(1)[rotated, OF _ Rep_wf_mbufn_map_tl[OF 1(2)] *])
+  case 2
+  then have *: "list_all2 R [Suc i..<j] (tl nts)"
+    by (auto simp: list.rel_sel[of R "[i..<j]" nts, simplified])
+  have [simp]: "Suc (i + (length nts - Suc 0)) = i + length nts" if "nts \<noteq> []"
+    using that by (fastforce simp flip: length_greater_0_conv)
+  with 2 show ?case
+    using Rep_wf_mbufn_in_set_Mini[OF 2(2)] Rep_wf_mbufn_notin_set[OF 2(2)]
+    by (subst (asm) Rep_mbufnt_take.simps) (force simp: Mini_def Rep_wf_mbufn_def
+        dest!: IH(2)[rotated, OF _ Rep_wf_mbufn_map_tl[OF 2(2)] *]
+        split: if_splits prod.splits)
+qed
+
+lemma Rep_mbufnt_take: "mbufnt_take f z buf nts = (z', buf', nts') \<Longrightarrow>  Rep_mbufnt_take f z (map Rep_mbuf_t buf) nts = (z', map Rep_mbuf_t buf', nts')"
+  sorry
 
 lemma mbufnt_take_eqD:
   assumes "mbufnt_take f z buf nts = (z', buf', nts')"
@@ -6129,29 +6320,8 @@ lemma mbufnt_take_eqD:
     and "k = Mini (i + length nts) js"
   shows "wf_mbufn k js Ps buf'"
     and "list_all2 R [k..<j] nts'"
-  using assms(1-4) unfolding assms(5)
-proof (induction f z buf nts arbitrary: i z' buf' nts' rule: mbufnt_take.induct)
-  case IH: (1 f z buf nts)
-  note mbufnt_take.simps[simp del]
-  case 1
-  then have *: "list_all2 R [Suc i..<j] (tl nts)"
-    by (auto simp: list.rel_sel[of R "[i..<j]" nts, simplified])
-  from 1 show ?case
-    using wf_mbufn_in_set_Mini[OF 1(2)]
-    by (subst (asm) mbufnt_take.simps)
-      (force simp: Mini_def wf_mbufn_def split: if_splits prod.splits elim!: list_all3_mono_strong
-        dest!: IH(1)[rotated, OF _ wf_mbufn_map_tl[OF 1(2)] *])
-  case 2
-  then have *: "list_all2 R [Suc i..<j] (tl nts)"
-    by (auto simp: list.rel_sel[of R "[i..<j]" nts, simplified])
-  have [simp]: "Suc (i + (length nts - Suc 0)) = i + length nts" if "nts \<noteq> []"
-    using that by (fastforce simp flip: length_greater_0_conv)
-  with 2 show ?case
-    using wf_mbufn_in_set_Mini[OF 2(2)] wf_mbufn_notin_set[OF 2(2)]
-    by (subst (asm) mbufnt_take.simps) (force simp: Mini_def wf_mbufn_def
-        dest!: IH(2)[rotated, OF _ wf_mbufn_map_tl[OF 2(2)] *]
-        split: if_splits prod.splits)
-qed
+  using Rep_mbufnt_take_eqD[OF Rep_mbufnt_take[OF assms(1)] assms(2)[folded Rep_wf_mbufn] assms(3-)]
+  by (auto simp: Rep_wf_mbufn[symmetric])
 
 lemma mbuf2t_take_list_induct:
   assumes "mbuf2t_list_take f z buf nts = (z', buf', nts')"
@@ -6198,15 +6368,15 @@ lemma list_all2_lastD:
   using assms list_all2_hdD(2)[OF assms, THEN less_imp_add_positive] unfolding list_all2_conv_all_nth
   by (auto dest!: spec[of _ "length xs - 1"] simp: last_conv_nth Suc_le_eq)
 
-lemma mbufn_take_induct[consumes 3, case_names base step]:
-  assumes "mbufn_take f z buf = (z', buf')"
-    and "wf_mbufn i js Ps buf"
+lemma Rep_mbufn_take_induct[consumes 3, case_names base step]:
+  assumes "Rep_mbufn_take f z buf = (z', buf')"
+    and "Rep_wf_mbufn i js Ps buf"
     and "U i z"
     and "\<And>k xs z. i \<le> k \<Longrightarrow> Suc k \<le> Mini i js \<Longrightarrow>
       list_all2 (\<lambda>P x. P k x) Ps xs \<Longrightarrow> U k z \<Longrightarrow> U (Suc k) (f xs z)"
   shows "U (Mini i js) z'"
-  using assms unfolding wf_mbufn_def
-proof (induction f z buf arbitrary: i z' buf' rule: mbufn_take.induct)
+  using assms unfolding Rep_wf_mbufn_def
+proof (induction f z buf arbitrary: i z' buf' rule: Rep_mbufn_take.induct)
   case rec: (1 f z buf)
   show ?case proof (cases "buf = []")
     case True
@@ -6233,7 +6403,7 @@ proof (induction f z buf arbitrary: i z' buf' rule: mbufn_take.induct)
         unfolding \<open>Mini i js = Mini (Suc i) js\<close>
       proof (rule rec.IH)
         show "\<not> (buf = [] \<or> [] \<in> set buf)" using nonempty False by simp
-        show "mbufn_take f (f (map hd buf) z) (map tl buf) = (z', buf')"
+        show "Rep_mbufn_take f (f (map hd buf) z) (map tl buf) = (z', buf')"
           using nonempty False rec.prems by simp
         show "list_all3 (\<lambda>P j xs. Suc i \<le> j \<and> list_all2 P [Suc i..<j] xs) Ps js (map tl buf)"
           using False rec.prems
@@ -6250,6 +6420,46 @@ proof (induction f z buf arbitrary: i z' buf' rule: mbufn_take.induct)
   qed
 qed
 
+lemma mbufn_take_induct[consumes 3, case_names base step]:
+  assumes "mbufn_take f z buf = (z', buf')"
+    and "wf_mbufn i js Ps buf"
+    and "U i z"
+    and "\<And>k xs z. i \<le> k \<Longrightarrow> Suc k \<le> Mini i js \<Longrightarrow>
+      list_all2 (\<lambda>P x. P k x) Ps xs \<Longrightarrow> U k z \<Longrightarrow> U (Suc k) (f xs z)"
+  shows "U (Mini i js) z'"
+  using Rep_mbufn_take_induct[OF Rep_mbufn_take[OF assms(1)] assms(2)[folded Rep_wf_mbufn] assms(3-)]
+  by auto
+
+lemma Rep_mbufnt_take_induct[consumes 5, case_names base step]:
+  assumes "Rep_mbufnt_take f z buf nts = (z', buf', nts')"
+    and "Rep_wf_mbufn i js Ps buf"
+    and "list_all2 R [i..<j] nts"
+    and "\<And>k. k \<in> set js \<Longrightarrow> k \<le> j"
+    and "U i z"
+    and "\<And>k xs t z. i \<le> k \<Longrightarrow> Suc k \<le> Mini j js \<Longrightarrow>
+      list_all2 (\<lambda>P x. P k x) Ps xs \<Longrightarrow> R k t \<Longrightarrow> U k z \<Longrightarrow> U (Suc k) (f xs t z)"
+  shows "U (Mini (i + length nts) js) z'"
+  using assms
+proof (induction f z buf nts arbitrary: i z' buf' nts' rule: Rep_mbufnt_take.induct)
+  case (1 f z buf nts)
+  then have *: "list_all2 R [Suc i..<j] (tl nts)"
+    by (auto simp: list.rel_sel[of R "[i..<j]" nts, simplified])
+  note mbufnt_take.simps[simp del]
+  from 1(2-6) have "i = Min (set js)" if "js \<noteq> []" "nts = []"
+    using that unfolding Rep_wf_mbufn_def using Rep_wf_mbufn_in_set_Mini[OF 1(3)]
+    by (fastforce simp: Mini_def list_all3_Cons neq_Nil_conv)
+  with 1(2-7) list_all2_hdD[OF 1(4)] show ?case
+    unfolding Rep_wf_mbufn_def using Rep_wf_mbufn_in_set_Mini[OF 1(3)] Rep_wf_mbufn_notin_set[OF 1(3)]
+    sorry
+(*
+    apply (subst (asm) Rep_mbufnt_take.simps)
+    apply (auto simp add: Mini_def list.rel_map Suc_le_eq
+        elim!: arg_cong2[of _ _ _ _ U, OF _ refl, THEN iffD1, rotated]
+        list_all3_mono_strong[THEN list_all3_list_all2I[of _ _ js]] list_all2_hdD
+        dest!: 1(1)[rotated, OF _ Rep_wf_mbufn_map_tl[OF 1(3)] * _ 1(7)] split: prod.split if_splits)
+*)
+qed
+
 lemma mbufnt_take_induct[consumes 5, case_names base step]:
   assumes "mbufnt_take f z buf nts = (z', buf', nts')"
     and "wf_mbufn i js Ps buf"
@@ -6259,23 +6469,8 @@ lemma mbufnt_take_induct[consumes 5, case_names base step]:
     and "\<And>k xs t z. i \<le> k \<Longrightarrow> Suc k \<le> Mini j js \<Longrightarrow>
       list_all2 (\<lambda>P x. P k x) Ps xs \<Longrightarrow> R k t \<Longrightarrow> U k z \<Longrightarrow> U (Suc k) (f xs t z)"
   shows "U (Mini (i + length nts) js) z'"
-  using assms
-proof (induction f z buf nts arbitrary: i z' buf' nts' rule: mbufnt_take.induct)
-  case (1 f z buf nts)
-  then have *: "list_all2 R [Suc i..<j] (tl nts)"
-    by (auto simp: list.rel_sel[of R "[i..<j]" nts, simplified])
-  note mbufnt_take.simps[simp del]
-  from 1(2-6) have "i = Min (set js)" if "js \<noteq> []" "nts = []"
-    using that unfolding wf_mbufn_def using wf_mbufn_in_set_Mini[OF 1(3)]
-    by (fastforce simp: Mini_def list_all3_Cons neq_Nil_conv)
-  with 1(2-7) list_all2_hdD[OF 1(4)] show ?case
-    unfolding wf_mbufn_def using wf_mbufn_in_set_Mini[OF 1(3)] wf_mbufn_notin_set[OF 1(3)]
-    by (subst (asm) mbufnt_take.simps)
-      (auto simp add: Mini_def list.rel_map Suc_le_eq
-        elim!: arg_cong2[of _ _ _ _ U, OF _ refl, THEN iffD1, rotated]
-        list_all3_mono_strong[THEN list_all3_list_all2I[of _ _ js]] list_all2_hdD
-        dest!: 1(1)[rotated, OF _ wf_mbufn_map_tl[OF 1(3)] * _ 1(7)] split: prod.split if_splits)
-qed
+  using Rep_mbufnt_take_induct[OF Rep_mbufnt_take[OF assms(1)] assms(2)[folded Rep_wf_mbufn] assms(3-)]
+  by auto
 
 lemma mbuf2_take_add':
   assumes eq: "mbuf2_take f (mbuf2_add xs ys buf) = (zs, buf')"
